otbn_model/spec/def.dfy
@@ -1,8 +1,10 @@
 // Trusted specification for the OpenTitan Bignum semantics
 
-datatype Bignum = Bignum(l7:uint32, l6:uint32, l5:uint32, l4:uint32, l3:uint32, l2:uint32, l1:uint32, l0:uint32)
+include "types.dfy"
 
 module bignum_def {
+
+import opened types
 
 // General purpose and control registers, 32b
 datatype Reg32 =
@@ -38,27 +40,27 @@ datatype ins32 =
 | ECALL // TODO
 
 datatype ins256 =
-| ADD(wrd:Reg256, wrs1:Reg256, wrs2:Reg256, shift_type:bool, shift_bytes:uint256, flg:bool)
-| ADDC(wrd:Reg256, wrs1:Reg256, wrs2:Reg256, shift_type:bool, shift_bytes:uint256, flg:bool)
-| ADDI(wrd:Reg256, wrs1:Reg256, imm:uint256, flg:bool)
+| ADD(wrd:Reg256, wrs1:Reg256, wrs2:Reg256, shift_type:bool, shift_bytes:Bignum, flg:bool)
+| ADDC(wrd:Reg256, wrs1:Reg256, wrs2:Reg256, shift_type:bool, shift_bytes:Bignum, flg:bool)
+| ADDI(wrd:Reg256, wrs1:Reg256, imm:Bignum, flg:bool)
 | ADDM(wrd:Reg256, wrs1:Reg256, wrs2:Reg256)
 | MULQACC
 | MULH(wrd:Reg256, wrs1:Reg256, hw1:bool, wrs2:Reg256, hw2:bool)
-| SUB(wrd:Reg256, wrs1:Reg256, wrs2:Reg256, shift_type:bool, shift_bytes:uint256, flg:bool)
-| SUBB(wrd:Reg256, wrs1:Reg256, wrs2:Reg256, shift_type:bool, shift_bytes:uint256, flg:bool)
-| SUBI(wrd:Reg256, wrs1:Reg256, imm:uint256, flg:bool)
+| SUB(wrd:Reg256, wrs1:Reg256, wrs2:Reg256, shift_type:bool, shift_bytes:Bignum, flg:bool)
+| SUBB(wrd:Reg256, wrs1:Reg256, wrs2:Reg256, shift_type:bool, shift_bytes:Bignum, flg:bool)
+| SUBI(wrd:Reg256, wrs1:Reg256, imm:Bignum, flg:bool)
 | SUBM(wrd:Reg256, wrs1:Reg256, wrs2:Reg256)
-| AND(wrd:Reg256, wrs1:Reg256, wrs2:Reg256, shift_type:bool, shift_bytes:uint256)
-| OR(wrd:Reg256, wrs1:Reg256, wrs2:Reg256, shift_type:bool, shift_bytes:uint256)
-| NOT(wrd:Reg256, wrs1:Reg256, wrs2:Reg256, shift_type:bool, shift_bytes:uint256)
-| XOR(wrd:Reg256, wrs1:Reg256, wrs2:Reg256, shift_type:bool, shift_bytes:uint256, flg:bool)
-| RSHI(wrd:Reg256, wrs1:Reg256, wrs2:Reg256, imm:uint256)
+| AND(wrd:Reg256, wrs1:Reg256, wrs2:Reg256, shift_type:bool, shift_bytes:Bignum)
+| OR(wrd:Reg256, wrs1:Reg256, wrs2:Reg256, shift_type:bool, shift_bytes:Bignum)
+| NOT(wrd:Reg256, wrs1:Reg256, wrs2:Reg256, shift_type:bool, shift_bytes:Bignum)
+| XOR(wrd:Reg256, wrs1:Reg256, wrs2:Reg256, shift_type:bool, shift_bytes:Bignum, flg:bool)
+| RSHI(wrd:Reg256, wrs1:Reg256, wrs2:Reg256, imm:Bignum)
 | SEL(wrd:Reg256, wrs1:Reg256, wrs2:Reg256, flg:bool)
 | CMP(wrs1:Reg256, wrs2:Reg256, flg:bool)
 | CMPB(wrs1:Reg256, wrs2:Reg256, flg:bool)
 | LID // TODO
 | SID // TODO
-| MOV(wrd:Reg256, wrs:uint256)
+| MOV(wrd:Reg256, wrs:Bignum)
 | MOVR // TODO
 | WSRRS // TODO
 | WSRRW // TODO
@@ -67,17 +69,93 @@ datatype codes = CNil | va_CCons(hd:code, tl:codes)
 
 datatype code =
 | Ins32(ins:ins32)
-| Ins256(ins:ins256)
+| Ins256(bn_ins:ins256)
 | Block(block:codes)
 
 type Frame = map<int, uint32>
 type Stack = seq<Frame>
 
 datatype state = state(
-	 xregs: map<Reg32, uint32>
-	 wregs: map<Reg256, Bignum>,
-	 flags: map<int, bool>,
+	 xregs: map<Reg32, uint32>, // 32-bit registers
+	 wregs: map<Reg256, Bignum>, // 256-bit registers
+	 //flags: map<int, bool>,
+	 stack: Stack,
 	 ok: bool)
 
+predicate IsUInt32(i:int) { 0 <= i < 0x1_0000_0000 }
+
+predicate ValidRegister32(xregs:map<Reg32, uint32>, r:Reg32)
+{
+	r in xregs
 }
 
+function eval_xreg(xregs:map<Reg32, uint32>, r:Reg32) : uint32
+{
+	if !ValidRegister32(xregs, r) then 24
+	else xregs[r]
+}
+
+predicate ValidRegisterIndex(index:int)
+{
+	0 <= index < 32
+}
+
+predicate ValidSourceRegister32(s:state, r:Reg32)
+{
+	if r.Rnd? then
+		ValidRegister32(s.xregs, r)
+	else
+		ValidRegister32(s.xregs, r) && ValidRegisterIndex(r.x)
+}
+
+predicate ValidDestinationRegister32(s:state, r:Reg32)
+{
+		!r.Rnd? && ValidRegister32(s.xregs, r) && ValidRegisterIndex(r.x)
+}
+
+function eval_reg32(s:state, r:Reg32) : uint32
+{
+	if !ValidSourceRegister32(s, r) then
+		42
+	else
+		s.xregs[r]
+}
+
+predicate evalIns32(xins:ins32, s:state, r:state)
+{
+	// TODO: actual implementation
+	if !s.ok then
+		!r.ok
+	else
+		r.ok
+}
+
+predicate evalIns256(wins:ins256, s:state, r:state)
+{
+	// TODO: actual implementation
+	if !s.ok then
+		!r.ok
+	else
+		r.ok
+}
+
+predicate evalBlock(block:codes, s:state, r:state)
+{
+    if block.CNil? then
+        r == s
+    else
+        exists r':state :: evalCode(block.hd, s, r') && evalBlock(block.tl, r', r)
+}
+
+predicate evalCode(c:code, s:state, r:state)
+    decreases c, 0
+{
+    match c
+        case Ins32(ins) => evalIns32(ins, s, r)
+        case Ins256(ins) => evalIns256(ins, s, r)
+        case Block(block) => evalBlock(block, s, r)
+        //case IfElse(cond, ifT, ifF) => evalIfElse(cond, ifT, ifF, s, r)
+        //case While(cond, body) => exists n:nat :: evalWhile(cond, body, n, s, r)
+}
+
+}
