otbn_model/spec/types.dfy
@@ -1,0 +1,28 @@
+module types {
+
+/////////////////
+// Native types
+/////////////////
+
+newtype{:nativeType "byte"} byte = i:int | 0 <= i < 0x100
+newtype{:nativeType "uint"} uint = i:int | 0 <= i < 0x1_0000_0000
+newtype{:nativeType "ulong"} ulong = i:int | 0 <= i < 0x1_0000_0000_0000_0000
+
+/////////////////
+// Subset types
+/////////////////
+
+type uint8   = i:int | 0 <= i < 0x100
+type uint16  = i:int | 0 <= i < 0x10000
+type uint32  = i:int | 0 <= i < 0x1_0000_0000
+type uint64  = i:int | 0 <= i < 0x1_0000_0000_0000_0000
+type uint128 = i:int | 0 <= i < 0x1_00000000_00000000_00000000_00000000
+type uint256 = i:int | 0 <= i < 0x1_0000000000000000_0000000000000000_0000000000000000_0000000000000000
+
+/////////////////
+// Bignum
+/////////////////
+	
+datatype Bignum = Bignum(l7:uint32, l6:uint32, l5:uint32, l4:uint32, l3:uint32, l2:uint32, l1:uint32, l0:uint32)
+
+} // end module types
